Prove interpret_sound.

AbstractDomain.v
@@ -1,6 +1,7 @@
 Require Export PolyAI.TotalMap.
 Require Export Coq.Sets.Ensembles.
 Require Import PolyAI.SSA.
+Require Import Coq.Program.Equality.
 
 Require Import String.
 Open Scope string_scope.
@@ -26,7 +27,7 @@ Class transfer_function {ab: Type} (A: adom ab) :=
       forall prog R l R' l' a inst,
         In RegisterMap (gamma a) R ->
         step prog (R, l) (R', l') ->
-        Some inst = List.nth_error prog l ->
+        inst = List.nth l prog (Const "X" 0) ->
         exists a', List.In (a', l') (transfer inst a l) /\
               In RegisterMap (gamma a') R'
   }.
@@ -53,4 +54,43 @@ Theorem interpret_compute_fixpoint {ab: Type} {A: adom ab} (T: transfer_function
              List.In (a', l') (transfer inst a l) ->
              le a' (List.nth l' a_dom top) = true.
 Proof.
-  Admitted.
+Admitted.
+
+
+Theorem interpret_sound {ab: Type} {A: adom ab} (T: transfer_function A) (prog: Program) :
+  forall R l, l < List.length prog ->
+         reachable_states prog (R, l) ->
+         In RegisterMap (gamma (List.nth l (interpret T prog) top)) R.
+Proof.
+  intros R l Hinbounds Hreachable.
+  inversion Hreachable.
+  subst.
+  generalize_eqs H.
+  generalize dependent l.
+  generalize dependent R.
+  generalize dependent R0.
+  induction H.
+  - intros.
+    apply JMeq_eq in H. injection H. intros.
+    apply JMeq_eq in H0. injection H0. intros.
+    subst.
+    pose proof (interpret_has_initial_state_top T p).
+    apply gamma_monotone in H1.
+    apply H1.
+    apply gamma_top.
+  - intros.
+    apply JMeq_eq in H1. apply JMeq_eq in H2. subst.
+    destruct s'.
+    inversion H0. subst.
+    pose proof H6 as Hl0.
+    apply (IHmulti_step R0 r) in H6; auto;
+      try (apply Reachable with (R := R0); auto).
+    pose proof (transfer_sound p r l0 R l) as H1.
+    apply H1 with (inst := (List.nth l0 p (Const "X" 0))) in H6; auto.
+    destruct H6. destruct H2.
+    pose proof (interpret_compute_fixpoint T p l0 l x).
+    apply H4 in Hl0; auto.
+    apply gamma_monotone in Hl0.
+    apply Hl0.
+    exact H3.
+Qed.
